updated to named_theorems; tuned;

thys/AWN/Inv_Cterms.thy
@@ -43,55 +43,18 @@ text {*
 
 lemma has_ctermsl: "p \<in> ctermsl \<Gamma> \<Longrightarrow> p \<in> ctermsl \<Gamma>" .
 
+named_theorems cterms_elimders "rules for truncating sequential process terms"
+named_theorems cterms_seqte "elimination rules for sequential process terms"
+named_theorems cterms_env "simplification rules for sequential process environments"
+named_theorems ctermsl_cases "destruction rules for case splitting ctermsl"
+named_theorems cterms_intros "introduction rules from cterms"
+named_theorems cterms_invs "invariants to try to apply at each vc"
+named_theorems cterms_final "elimination rules to try on each vc after simplification"
+
 ML {*
-structure CtermsElimders = Named_Thms
-  (val name = @{binding "cterms_elimders"}
-   val description = "Rules for truncating sequential process terms")
-val cterms_elimders_add = Thm.declaration_attribute CtermsElimders.add_thm
-val cterms_elimders_del = Thm.declaration_attribute CtermsElimders.del_thm
-
-structure CtermsTE = Named_Thms
-  (val name = @{binding "cterms_seqte"}
-   val description = "Elimination rules for sequential process terms")
-val cterms_seqte_add = Thm.declaration_attribute CtermsTE.add_thm
-val cterms_seqte_del = Thm.declaration_attribute CtermsTE.del_thm
-
-structure CtermsEnvRules = Named_Thms
-  (val name = @{binding "cterms_env"}
-   val description = "Simplification rules for sequential process environments")
-val cterms_env_add = Thm.declaration_attribute CtermsEnvRules.add_thm
-val cterms_env_del = Thm.declaration_attribute CtermsEnvRules.del_thm
-
-structure CtermslCases = Named_Thms
-  (val name = @{binding "ctermsl_cases"}
-   val description = "Destruction rules for case splitting ctermsl")
-val ctermsl_cases_add = Thm.declaration_attribute CtermslCases.add_thm
-val ctermsl_cases_del = Thm.declaration_attribute CtermslCases.del_thm
-
-structure CtermsIntros = Named_Thms
-  (val name = @{binding "cterms_intros"}
-   val description = "Introduction rules from cterms")
-val cterms_intros_add = Thm.declaration_attribute CtermsIntros.add_thm
-val cterms_intros_del = Thm.declaration_attribute CtermsIntros.del_thm
-
-structure CtermsInvs = Named_Thms
-  (val name = @{binding "cterms_invs"}
-   val description = "Invariants to try to apply at each vc")
-val cterms_invs_add = Thm.declaration_attribute CtermsInvs.add_thm
-val cterms_invs_del = Thm.declaration_attribute CtermsInvs.del_thm
-
-structure CtermsFinal = Named_Thms
-  (val name = @{binding "cterms_final"}
-   val description = "Elimination rules to try on each vc after simplification")
-val cterms_final_add = Thm.declaration_attribute CtermsFinal.add_thm
-val cterms_final_del = Thm.declaration_attribute CtermsFinal.del_thm
-
 fun simp_only thms ctxt =
   asm_full_simp_tac
-     (Context.proof_map
-        (Simplifier.map_ss (Raw_Simplifier.clear_simpset
-                            #> fold Simplifier.add_simp thms))
-        ctxt)
+     (ctxt |> Raw_Simplifier.clear_simpset |> fold Simplifier.add_simp thms)
 
 (* shallow_simp is useful for mopping up assumptions before really trying to simplify.
    Perhaps surprisingly, this saves minutes in some of the proofs that use a lot of
@@ -102,8 +65,8 @@ fun shallow_simp ctxt =
   end
 
 fun create_vcs ctxt i =
-  let val main_simp_thms =  CtermsEnvRules.get ctxt
-      val ctermsl_cases = CtermslCases.get ctxt
+  let val main_simp_thms = rev (Named_Theorems.get ctxt @{named_theorems cterms_env})
+      val ctermsl_cases = rev (Named_Theorems.get ctxt @{named_theorems ctermsl_cases})
   in
     dtac @{thm has_ctermsl} i
     THEN_ELSE (dmatch_tac ctermsl_cases i
@@ -117,23 +80,24 @@ fun create_vcs ctxt i =
   end
 
 fun try_invs ctxt =
-  let val inv_thms =  CtermsInvs.get ctxt
+  let val inv_thms = rev (Named_Theorems.get ctxt @{named_theorems cterms_invs})
       fun fapp thm = TRY o (EVERY' (ftac thm :: replicate (Thm.nprems_of thm - 1) assume_tac))
   in
     EVERY' (map fapp inv_thms)
   end
 
 fun try_final ctxt =
-  let val final_thms =  CtermsFinal.get ctxt
+  let val final_thms = rev (Named_Theorems.get ctxt @{named_theorems cterms_final})
       fun eapp thm = EVERY' (etac thm :: replicate (Thm.nprems_of thm - 1) assume_tac)
   in
     TRY o (FIRST' (map eapp final_thms))
   end
 
 fun each ctxt =
-  (EVERY' ((ematch_tac (CtermsElimders.get ctxt) :: replicate 2 assume_tac))
+  (EVERY' ((ematch_tac (rev (Named_Theorems.get ctxt @{named_theorems cterms_elimders})) ::
+    replicate 2 assume_tac))
    THEN' simp_only @{thms labels_psimps} ctxt
-   THEN' (ematch_tac (CtermsTE.get ctxt)
+   THEN' (ematch_tac (rev (Named_Theorems.get ctxt @{named_theorems cterms_seqte}))
      THEN_ALL_NEW
        (fn j => simp_only [@{thm mem_Collect_eq}] ctxt j
                   THEN REPEAT (etac @{thm exE} j)
@@ -151,7 +115,7 @@ fun simp_all ctxt =
   end
 
 fun intro_and_invs ctxt i =
-  let val cterms_intros = CtermsIntros.get ctxt in
+  let val cterms_intros = rev (Named_Theorems.get ctxt @{named_theorems cterms_intros}) in
     match_tac cterms_intros i
     THEN (PARALLEL_GOALS (ALLGOALS (try_invs ctxt)))
   end
@@ -159,35 +123,30 @@ fun intro_and_invs ctxt i =
 fun process_vcs ctxt _ =
   ALLGOALS (create_vcs ctxt ORELSE' (SOLVED' (clarsimp_tac ctxt)))
   THEN (PARALLEL_GOALS (ALLGOALS (TRY o (each ctxt))))
+*}
 
-val intro_onlyN = "intro_only"
-val vcs_onlyN = "vcs_only"
-val invN = "inv"
-val solveN = "solve"
+method_setup inv_cterms = {*
+  let
+    val intro_onlyN = "intro_only"
+    val vcs_onlyN = "vcs_only"
+    val invN = "inv"
+    val solveN = "solve"
 
-val inv_cterms_options =
-  (Args.parens (Args.$$$ intro_onlyN) >>  K intro_and_invs ||
-   Args.parens (Args.$$$ vcs_onlyN) >>  K (fn ctxt => intro_and_invs ctxt
-                                                      THEN' process_vcs ctxt) ||
-   Scan.succeed (fn ctxt => intro_and_invs ctxt
-                            THEN' process_vcs ctxt
-                            THEN' K (simp_all ctxt)))
-
-val inv_cterms_setup =
-  Method.setup @{binding inv_cterms}
+    val inv_cterms_options =
+      (Args.parens (Args.$$$ intro_onlyN) >>  K intro_and_invs ||
+       Args.parens (Args.$$$ vcs_onlyN) >>  K (fn ctxt => intro_and_invs ctxt
+                                                          THEN' process_vcs ctxt) ||
+       Scan.succeed (fn ctxt => intro_and_invs ctxt
+                                THEN' process_vcs ctxt
+                                THEN' K (simp_all ctxt)))
+  in
     (Scan.lift inv_cterms_options --| Method.sections
-      ((Args.$$$ invN -- Args.add -- Args.colon >> K (I, cterms_invs_add))
-       :: (Args.$$$ solveN -- Args.colon >> K (I, cterms_final_add))
+      ((Args.$$$ invN -- Args.add -- Args.colon >> K (I, Named_Theorems.add @{named_theorems cterms_invs}))
+       :: (Args.$$$ solveN -- Args.colon >> K (I, Named_Theorems.add @{named_theorems cterms_final}))
        :: Simplifier.simp_modifiers)
       >> (fn tac => SIMPLE_METHOD' o tac))
-    "Solve invariants by considering all (interesting) control terms."
-*}
-attribute_setup cterms_seqte    = {* Attrib.add_del cterms_seqte_add cterms_seqte_del *}
-attribute_setup cterms_elimders = {* Attrib.add_del cterms_elimders_add cterms_elimders_del *}
-attribute_setup cterms_env =      {* Attrib.add_del cterms_env_add cterms_env_del *}
-attribute_setup ctermsl_cases =   {* Attrib.add_del ctermsl_cases_add ctermsl_cases_del *}
-attribute_setup cterms_intros =   {* Attrib.add_del cterms_intros_add cterms_intros_del *}
-setup {* inv_cterms_setup *}
+  end
+*} "solve invariants by considering all (interesting) control terms"
 
 declare
   insert_iff [cterms_env]                                                
